WIP type translation mostly done

translation/Translation.v
@@ -1,5 +1,135 @@
 Require Import Predefs.
 Require Import TLC.LibTactics.
+Require Import TLC.LibLN.
+Require Import GMu.Prelude.
+Require Import Definitions.
+
+(*
+*** Warning: in file Predefs.v, 
+    required library Definitions matches several files in path
+    (found Definitions.v in ../lambda2Gmu and ../../dot-calculus/src/extensions/paths; used the latter)
+*)
+
+(* TODO can we instantiate this? Or maybe we don't need to? *)
+Axiom Unit : typ_label.
+Axiom Tuple : typ_label.
+Axiom GenT : typ_label.
+Axiom Ai : nat -> typ_label.
+Axiom Bi : nat -> typ_label.
+Axiom GN : Source.GADTName -> typ_label.
+
+Definition refLibTyp (name : typ_label) (offset : nat) : Target.typ.
+  apply typ_path.
+  - constructor.
+    + apply avar_b. exact offset.
+    + apply nil.
+  - exact name.
+Defined.
+
+Definition UnitT (offset : nat) : Target.typ :=
+  refLibTyp Unit offset.
+
+Definition TupleT (offset : nat) (T1 T2 : Target.typ) : Target.typ.
+Admitted.
+
+Definition GenArgT : Target.typ :=
+  typ_rcd { GenT >: ⊥ <: ⊤ }.
+
+Fixpoint translateType (T : Source.typ) (offset : nat) : Target.typ.
+  destruct T as []eqn:H.
+  - (* bvar *)
+    apply typ_path.
+    + constructor.
+      * exact (avar_b n).
+      * exact nil.
+    + apply GenT.
+  - (* fvar *)
+    exact (typ_path (pvar v) GenT).
+  - (* unit *)
+    exact (UnitT offset).
+  - (* tuple *)
+    refine (let T1 := translateType t1 offset in _).
+    refine (let T2 := translateType t2 offset in _).
+    exact (TupleT offset T1 T2).
+  - (* ==> *)
+    refine (let T1 := translateType t1 offset in _).
+    refine (let T2 := translateType t2 (1+offset) in _).
+    exact (typ_all T1 T2).
+  - (* forall *)
+    refine (let T1 := translateType t (1+offset) in _).
+    exact (typ_all GenArgT T1).
+  - (* GADT *)
+    refine (let Ts := List.map (fun t => translateType t offset) l in _).
+    refine (let base := typ_path (p_sel (avar_b offset) nil) (GN g) in _).
+    refine (let Ts2 :=
+                List.fold_left
+                  (fun acc T => match acc with
+                             | (i, rest) =>
+                               (
+                                 1+i,
+                                 (rest ∧ typ_rcd { Ai i >: ⊥ <: ⊤ })
+                               )
+                             end)
+                  Ts
+                  (1, base)
+            in _).
+    destruct Ts2 as []eqn:Heq.
+    exact t.
+Defined.
+
+Definition translateTyp0 (T : Source.typ) : Target.typ := translateType T 0.
+
+Definition translateEnv (Σ : Source.GADTEnv) : Target.trm.
+Admitted.
+
+Axiom envId : var. (* TODO? *)
+
+Inductive TypedTrm : Set :=. (*TODO*)
+
+Fixpoint translateTerm (Σ : Source.GADTEnv) (typenv : list Target.typ) (trmenv : list Target.trm) (t : TypedTrm) : Target.trm.
+Admitted.
+
+Definition translateProgram (Σ : Source.GADTEnv) (main : TypedTrm) : Target.trm.
+Admitted.
+
+Fixpoint forget (t : TypedTrm) : Source.trm.
+Admitted.
+
+Import Source.
+Axiom typinga : typing_taint -> GADTEnv -> typctx -> ctx -> TypedTrm -> typ -> Prop.
+Definition typ_from_trm (tt : TypedTrm) : typ.
+Admitted.
+
+Lemma typing_gives_types : forall Σ Δ E t T,
+    {Σ, Δ, E} ⊢(Tgen) t ∈ T ->
+    exists tt, forget tt = t /\ typinga Tgen Σ Δ E tt T.
+Admitted.
+
+Lemma forgetting_preserves_typing : forall Σ Δ E tt T,
+    typinga Tgen Σ Δ E tt T ->
+    typing Tgen Σ Δ E (forget tt) T.
+Admitted.
+
+Definition translation2 : forall Σ Δ E t T,
+    {Σ, Δ, E} ⊢(Tgen) t ∈ T ->
+    Target.trm.
+  intros.
+  induction t.
+Admitted.
+
+Lemma translation_correct : forall Σ Δ E t T,
+    forall (TT : {Σ, Δ, E} ⊢(Tgen) t ∈ T),
+      Target.ty_trm empty (translation2 Σ Δ E t T TT) (translateTyp0 T).
+Admitted.
+
+Lemma translation_same : forall Σ Δ E ta T,
+    forall (TT : {Σ, Δ, E} ⊢(Tgen) (forget ta) ∈ T),
+      translateProgram Σ ta = translation2 Σ Δ E (forget ta) T TT.
+Admitted.
+
+Lemma translation_set_correct : forall (),
+
+
 
 (* lemma from https://stackoverflow.com/q/27322979/1296238 *)
 Lemma ex_falso: forall T: Type, False -> T.
