translation/Predefs.v
@@ -21,49 +21,50 @@ End Target.
 Inductive typed_target_term : Set :=
   typed_target_term_cons : forall (t : Target.trm) (T : Target.typ) (Htyp : Target.ty_trm empty t T), typed_target_term.
 
-(*
-The translation function is supposed to take a source typing derivation and return a typing derivation of analogous term in the target language. Thus, such a definition is also a proof of typing-preservation of the translation.
-*)
-Definition translation_type :=
-  forall (Σ : Source.GADTEnv)
-    (t : Source.trm) (T : Source.typ)
-    (Henv : Source.okGadt Σ)
-    (Htyp : Source.typing Σ empty t T),
-    typed_target_term.
-
 Definition get_term (R : typed_target_term) : Target.trm :=
   match R with
   | typed_target_term_cons t _ _ => t
   end.
 
+(*
+The translation function is supposed to take a source typing derivation and return a typing derivation of analogous term in the target language. Thus, such a definition is also a proof of typing-preservation of the translation.
+*)
+(* Definition translation_type := *)
+(*   forall (Σ : Source.GADTEnv) *)
+(*     (t : Source.trm) (T : Source.typ) *)
+(*     (Henv : Source.okGadt Σ) *)
+(*     (Htyp : Source.typing Σ empty t T), *)
+(*     exists pTT : typed_target_term,  . *)
+
+
 (* TODO: we will probably decouple translation of Source.GADTEnv from translation of terms, we may also decouple them in this definition ? *)
 
-Section translation_semantics.
-  Variable translator : translation_type.
+(* Section translation_semantics. *)
+(*   Variable translator : translation_type. *)
 
-  Definition target_evaluates := Target.star Target.red.
-  (* This may likely change.
-  The initial idea is to say that for every reduction in the source calculus, we can find an analogous series of reductions in the target *)
-  Definition translation_preserves_semantics :=
-    forall (Σ : Source.GADTEnv)
-      (ts : Source.trm) (Ts : Source.typ)
-      (ts' : Source.trm)
-      (Henv : Source.okGadt Σ)
-      (Htyp : Source.typing Σ empty ts Ts)
-      (R : typed_target_term)
-      (Htranslates : translator Σ ts Ts Henv Htyp = R)
-      (Htyp' : Source.typing Σ empty ts' Ts)
-      (HsrcRed : Source.red ts ts'),
-    exists (γ γ' : Target.sta) (* TODO handling the stores, may have to happen inside translation???? *)
-      (R' : typed_target_term),
-      translator Σ ts' Ts Henv Htyp' = R' /\
-      target_evaluates (γ, get_term R) (γ', get_term R').
+(*   Definition target_evaluates := Target.star Target.red. *)
+(*   (* This may likely change. *)
+(*   The initial idea is to say that for every reduction in the source calculus, we can find an analogous series of reductions in the target *) *)
+(*   Definition translation_preserves_semantics := *)
+(*     forall (Σ : Source.GADTEnv) *)
+(*       (ts : Source.trm) (Ts : Source.typ) *)
+(*       (ts' : Source.trm) *)
+(*       (Henv : Source.okGadt Σ) *)
+(*       (Htyp : Source.typing Σ empty ts Ts) *)
+(*       (R : typed_target_term) *)
+(*       (Htranslates : translator Σ ts Ts Henv Htyp = R) *)
+(*       (Htyp' : Source.typing Σ empty ts' Ts) *)
+(*       (HsrcRed : Source.red ts ts'), *)
+(*     exists (γ γ' : Target.sta) (* TODO handling the stores, may have to happen inside translation???? *) *)
+(*       (R' : typed_target_term), *)
+(*       translator Σ ts' Ts Henv Htyp' = R' /\ *)
+(*       target_evaluates (γ, get_term R) (γ', get_term R'). *)
 
-  (* another approach could be to characterize just the looping or final values *)
-  (* something like:
-     forall ts,
-            ts loops -> (translate ts) loops
-         /\ ts endswithval v -> (translate ts) ends with val v' /\ (translateVal v = v')
-  *)
+(*   (* another approach could be to characterize just the looping or final values *) *)
+(*   (* something like: *)
+(*      forall ts, *)
+(*             ts loops -> (translate ts) loops *)
+(*          /\ ts endswithval v -> (translate ts) ends with val v' /\ (translateVal v = v') *)
+(*   *) *)
 
-End translation_semantics.
+(* End translation_semantics. *)
